Start proving non-trivial spec for idutil

new/proof/go_etcd_io/etcd/pkg/v3/idutil.v
@@ -1,3 +1,4 @@
+From coqutil Require Import Z.bitblast.
 Require Export New.generatedproof.go_etcd_io.etcd.pkg.v3.idutil.
 Require Export New.proof.proof_prelude.
 From New.proof Require Import time math sync.atomic.
@@ -9,54 +10,105 @@ Context `{!globalsGS Σ} {go_ctx : GoContext}.
 #[global] Instance : IsPkgInit math := define_is_pkg_init True%I.
 #[global] Instance : IsPkgInit idutil := define_is_pkg_init True%I.
 
-Definition is_Generator (g : loc) : iProp Σ :=
-  ∃ (prefix : w64),
-    "#prefix" ∷ g ↦s[idutil.Generator :: "prefix"]□ prefix ∗
-    "#suffix" ∷ inv nroot (∃ (suffix : w64),
-          struct.field_ref_f idutil.Generator "suffix" g ↦ suffix
+(* FIXME: id.go says that the overflowing of cnt into timestamp is intentional
+   "to extend the event window to 2^56". However, I only count 48 bits. Is that
+   a typo? *)
+Definition is_Generator (g : loc) (R : w64 → iProp Σ) : iProp Σ :=
+  ∃ (prefix : Z),
+    "#prefix" ∷ g ↦s[idutil.Generator :: "prefix"]□ (W64 (prefix * 2^48)) ∗
+    "#Hinv" ∷
+      inv nroot (∃ (init num_used : Z),
+          "suffix" ∷ struct.field_ref_f idutil.Generator "suffix" g ↦ W64 (init + num_used) ∗
+          "HR" ∷ ([∗ list] i ∈ seqZ (init + num_used + 1) (2^48 - num_used),
+                    R (W64 (prefix * 2^48 + i `mod` 2^48)))
       ) ∗
     "_" ∷ True.
 #[global] Opaque is_Generator.
 #[local] Transparent is_Generator.
-Instance : ∀ s, Persistent (is_Generator s).
+#[global] Instance : ∀ s R, Persistent (is_Generator s R).
 Proof. apply _. Qed.
 
-Lemma wp_lowbit (x n : w64) :
+(* Specialized to 48 low bits. *)
+#[local]
+Lemma wp_lowbit (x : w64) :
   {{{ is_pkg_init idutil }}}
-    @! idutil.lowbit #x #n
-  {{{ (y : w64), RET #y; True }}}.
+    @! idutil.lowbit #x #(W64 48)
+  {{{ RET #(W64 ((uint.Z x) `mod` 2^(uint.Z 48))); True }}}.
 Proof.
-  wp_start. wp_auto. iApply "HΦ". done.
+  wp_start as "%H". wp_auto.
+  iSpecialize ("HΦ" with "[//]").
+  iExactEq "HΦ". f_equal. f_equal.
+  rewrite Automation.word.word_eq_iff_Z_eq.
+  rewrite word.unsigned_and Automation.word.unsigned_sru'. 2:{ word. }
+  repeat ereplace (uint.Z (W64 ?[a])) with (?a) by word.
+  replace (uint.Z (word.sub (W64 _) _)) with (64 - 48)%Z by word.
+  replace (_ `div` _) with (Z.ones (uint.Z 48)).
+  2:{ vm_compute Z.ones. unfold math.MaxUint64. word. }
+  rewrite Z.land_ones //. word.
 Qed.
 
-Lemma wp_Generator__Next g :
-  {{{ is_pkg_init idutil ∗ is_Generator g }}}
+Lemma wp_Generator__Next g R :
+  {{{ is_pkg_init idutil ∗ is_Generator g R }}}
     g @ (ptrT.id idutil.Generator.id) @ "Next" #()
-  {{{ (i : w64), RET #i; True }}}.
+  {{{ (i : w64), RET #i; R i }}}.
 Proof.
-  wp_start as "H". iNamedSuffix "H" "_g".
-  wp_auto. wp_bind.
+  wp_start as "H". iNamed "H". wp_auto_lc 1. wp_bind.
   wp_apply wp_AddUint64.
-  iInv "suffix_g" as ">Hi" "Hclose".
+  iInv "Hinv" as "Hi" "Hclose".
+  iMod (lc_fupd_elim_later with "[$] Hi") as "Hi". iNamedSuffix "Hi" "_inv".
   iApply fupd_mask_intro. { solve_ndisj. } iIntros "Hmask".
-  iNamed "Hi". iFrame. iIntros "Hi".
-  iMod "Hmask". iMod ("Hclose" with "[$Hi]") as "_". iModIntro.
-  wp_auto. wp_apply wp_lowbit as "%y _". iApply "HΦ". done.
-Qed.
+  iFrame. iIntros "suffix_inv".
+  ereplace (word.add ?[a] ?[b]) with (W64 (init + (num_used + 1))) by word.
+  rewrite seqZ_cons.
+  2:{ admit. } (* TODO: requires knowing that there are fewer than 2^56 calls to [Next]. *)
+  iDestruct "HR_inv" as "[HR HR_inv]".
+  iMod "Hmask". iMod ("Hclose" with "[suffix_inv HR_inv]") as "_".
+  {
+    ereplace (Z.succ (?[a] + ?[b] + 1)) with (?a + (?b + 1) + 1) by word.
+    ereplace (Z.pred (?[a] - ?[b])) with (?a - (?b + 1)) by word.
+    iFrame.
+  }
+  iModIntro.
+  wp_auto.
+  wp_apply wp_lowbit. iApply "HΦ".
+  iExactEq "HR". f_equal.
+  rewrite Automation.word.word_eq_iff_Z_eq.
+  rewrite word.unsigned_or.
+  rewrite -Z.add_nocarry_lor.
+  2:{
+    Z.bitblast.
+    destruct (decide (i < 48)).
+    - apply andb_false_intro1.
+      rewrite Z.testbit_mod_pow2 // Z.mul_pow2_bits_low //. lia.
+    - apply andb_false_intro2.
+      ereplace (uint.Z (W64 ?[a])) with ?a by word.
+      rewrite Z.testbit_mod_pow2 //.
+      apply andb_false_intro1. word.
+  }
+  word.
+Admitted. (* overflow *)
 
-Lemma wp_NewGenerator (memberID : w16) (now : time.Time.t) :
-  {{{ is_pkg_init idutil }}}
+(* TODO: this is overly conservative. Really should only demand [R] for the
+   range of IDs with future timestamps, since the old ones might've been used
+   before a crash+restart. *)
+Lemma wp_NewGenerator R (memberID : w16) (now : time.Time.t) :
+  {{{
+      is_pkg_init idutil ∗
+      ([∗ list] i ∈ seqZ 0 (2^64), R (W64 i))
+  }}}
     @! idutil.NewGenerator #memberID #now
-  {{{ g, RET #g; is_Generator g }}}.
+  {{{ g, RET #g; is_Generator g R }}}.
 Proof.
-  wp_start as "H". wp_auto.
+  wp_start as "HR". wp_auto.
   wp_apply wp_Time__UnixNano as "%nowNano _".
-  wp_apply wp_lowbit as "% _". wp_alloc g as "Hg".
+  (* FIXME: wp_lowbit should *at least* support `suffixLen` and `tsLen` *)
+  (*
+  wp_apply wp_lowbit. wp_alloc g as "Hg".
   iApply wp_fupd. wp_auto. iApply "HΦ". iFrame "∗#".
   iDestruct (struct_fields_split with "Hg") as "Hg". iNamed "Hg".
   iPersist "Hprefix". iFrame "#".
   iMod (inv_alloc with "[Hsuffix]") as "$"; last done.
-  iFrame.
-Qed.
+  iFrame. *)
+Admitted.
 
 End wps.
